proof/agp32CorrectScript.sml
@@ -12,13 +12,11 @@ val _ = guess_lengths ();
 
 (* Init relation implies Rel at cycle 0 *)
 Theorem agp32_Init_implies_Rel:
-  !k fext fbits s a I.
-    k >= 1 ==>
-    k <= 5 ==>
+  !fext fbits s a I.
     s = agp32 fext fbits ==>
-    I(k,0) = 0 ==>
+    (!k.I(k,0) = 0) ==>
     Init (fext 0) (s 0) a ==>
-    Rel (fext 0) (s 0) I 0 a 0
+    Rel I (fext 0) (s 0) a 0
 Proof
   rpt strip_tac >>
   fs [Init_def,Rel_def] >> rw [] >-
@@ -28,9 +26,7 @@ QED
 
 (* correctness of the pipelined Silver concerning the ISA *)
 Theorem agp32_Rel_ag32_correct:
-  !k fext fbits s a (t:num) I C.
-    k >= 1 ==>
-    k <= 5 ==>
+  !fext fbits s a (t:num) I C.
     s = agp32 fext fbits ==>
     (!t. SC_self_mod (s t)) ==>
     is_mem fext_accessor_circuit s fext ==>
@@ -38,35 +34,45 @@ Theorem agp32_Rel_ag32_correct:
     is_interrupt_interface fext_accessor_circuit s fext ==>
     is_data_in fext ==>
     (* cache oracle can introduce hit/miss *)
-    (!t. C (s t).data_addr (s t).data_wstrb (s t).data_wdata (s t).command (s t).PC <=> (fext t).ready) ==>
+    (!t. C (s t).data_addr (s t).data_wstrb (s t).data_wdata (s t).command (s t).PC
+         <=> (fext t).ready) ==>
     Init (fext 0) (s 0) a ==>
     (** properties of scheduling function I **)
+    (!k.I(k,0) = 0) ==>
     (!t k. enable_stg k (s (SUC t)) ==> I(k,SUC t) = I(k,t) + 1) ==>
-    I(k,0) = 0 ==>
-    Rel (fext t) (s t) I t a (I(k,t))
+    Rel I (fext t) (s t) a t
 Proof
   Induct_on `t` >>
   rpt strip_tac >-
    METIS_TAC [agp32_Init_implies_Rel] >>
-  `Rel (fext t) (s t) I' t a (I' (k,t))` by METIS_TAC [] >>
-  Q.ABBREV_TAC `i = I'(k,t)` >> 
-  Cases_on `enable_stg k (s (SUC t))` >-
-   (`I'(k, SUC t) = SUC i` by fs [] >> fs [Rel_def] >>
-    Cases_on `k = 1` >-
-     (** IF stage **)
-     (fs [] >> rw [] >-
-       fs [GSYM ag32_data_in_unchanged,is_data_in_def] >>
-      `I'(1,SUC t) <> I'(2,SUC t)` by cheat >> fs [] >>
-      `I'(1,SUC t) <> I'(3,SUC t)` by cheat >> fs [] >>
-      `I'(1,SUC t) <> I'(4,SUC t)` by cheat >> fs [] >>
-      `I'(1,SUC t) <> I'(5,SUC t)` by cheat >> fs [] >>
-      rw [IF_Rel_def] >>
-      `?s s'. (agp32 fext fbits (SUC t)).IF.IF_instr =
-      (IF_instr_update (fext (SUC t)) s s').IF.IF_instr`
-        by rw [agp32_IF_instr_updated_by_IF_instr_update] >>
-      rw [IF_instr_update_def,instr_def] >> cheat) >>
+  `Rel I' (fext t) (s t) a t` by METIS_TAC [] >>
+  fs [Rel_def] >> rw [] >-
+     (** data_in **)
+   fs [is_data_in_def,ag32_data_in_unchanged_all] >-
+     (** carryflag **)
+   cheat >-
+   (** overflow flag **)
+   cheat >-
+   (** PC when jump **)
+   cheat >-
+   (** PC when not jump **)
+   cheat >-
+   (** memory **)
+   cheat >-
+   (** data_out **)
+   cheat >-
+   (** registers **)
+   cheat >-
+   (** invisiable regs in IF **)
+   (rw [IF_Rel_def] >-
+    (** IF_instr when memory is ready **)
+    (`?s s'. (agp32 fext fbits (SUC t)).IF.IF_instr =
+     (IF_instr_update (fext (SUC t)) s s').IF.IF_instr`
+       by rw [agp32_IF_instr_updated_by_IF_instr_update] >>
+     rw [IF_instr_update_def,instr_def] >> cheat) >>
+    (** IF_instr when not ready **)
     cheat) >>
-  cheat
+  cheat         
 QED
 
 val _ = export_theory ();
